lakefile.lean
@@ -5,7 +5,7 @@ package «lido-srv3-proof-closure» where
   version := v!"0.1.0"
 
 require verity from git
-  "https://github.com/lfglabs-dev/verity.git"@"33722270d996c7a3a520a71ecee42d7d232da100"
+  "https://github.com/lfglabs-dev/verity.git"@"538c4a9ce2baa25b56062bdc727eb0191ad9e67f"
 
 @[default_target]
 lean_lib «LidoSRv3» where
